src/Ren.v
@@ -1,4 +1,5 @@
 Require Export
+  Coq.Program.Equality
   Ty
   Exp.
 
@@ -11,111 +12,157 @@ Import ListNotations.
 
 Section Ren.
 
-Definition Ren Γ Γ' := ∀ τ, Var Γ τ → Var Γ' τ.
+Inductive Ren : Env → Env → Type :=
+  | NoRen : Ren [] []
+  | Drop {τ Γ Γ'} : Ren Γ Γ' → Ren (τ :: Γ) Γ'
+  | Keep {τ Γ Γ'} : Ren Γ Γ' → Ren (τ :: Γ) (τ :: Γ').
 
-Definition idRen {Γ} : Ren Γ Γ := λ _, id.
+Derive Signature NoConfusion for Ren.
 
-Definition tlRen {Γ Γ' τ} (r : Ren (τ :: Γ) Γ') : Ren Γ Γ' :=
-  fun τ' v => r τ' (SV v).
-Definition hdRen {Γ Γ' τ} (r : Ren (τ :: Γ) Γ') : Var Γ' τ := r τ ZV.
+Fixpoint idRen {Γ} : Ren Γ Γ :=
+  match Γ with
+  | []     => NoRen
+  | τ :: Γ => Keep idRen
+  end.
 
-Definition skip1 {Γ τ} : Ren Γ (τ :: Γ) := λ _, SV.
+Lemma Keep_idRen {Γ τ} : Keep (τ:=τ) (@idRen Γ) = idRen.
+Proof. now induction Γ. Qed.
 
-Equations skipn {Γ} Γ' : Ren Γ (Γ' ++ Γ) :=
-  skipn []        := λ _, id;
-  skipn (x :: xs) := λ τ v, SV (skipn xs τ v).
+Corollary NoRen_idRen : NoRen = idRen.
+Proof. reflexivity. Qed.
 
-Equations RTmL {Γ Γ' τ} (r : Ren Γ Γ')
-          (* Ren (τ :: Γ) (τ :: Γ') *)
-          τ' (v : Var (τ :: Γ) τ') : Var (τ :: Γ') τ' :=
-  RTmL r τ' ZV      := ZV;
-  RTmL r τ' (SV v') := SV (r _ v').
+Definition skip1 {Γ τ} : Ren (τ :: Γ) Γ := Drop idRen.
 
-Lemma RTmL_id {Γ τ} : @RTmL Γ Γ τ (λ _, id) = λ _, id.
+Equations RcR {Γ Γ' Γ''} (r : Ren Γ' Γ'') (r' : Ren Γ Γ') : Ren Γ Γ'' :=
+  RcR σ        NoRen    := σ;
+  RcR σ        (Drop δ) := Drop (RcR σ δ);
+  RcR (Drop σ) (Keep δ) := Drop (RcR σ δ);
+  RcR (Keep σ) (Keep δ) := Keep (RcR σ δ).
+
+Lemma RcR_idRen_left {Γ Γ'} (σ : Ren Γ Γ') :
+  RcR idRen σ = σ.
 Proof.
-  extensionality τ'.
-  extensionality v.
-  dependent elimination v.
-  - now rewrite RTmL_equation_1.
-  - now rewrite RTmL_equation_2.
+  induction σ; simp RcR; simpl; simp RcR; auto;
+  now rewrite IHσ.
 Qed.
 
-Definition RcR {Γ Γ' Γ''} (r : Ren Γ' Γ'') (r' : Ren Γ Γ') :=
-  (λ τ v, r τ (r' τ v)) : Ren Γ Γ''.
-
-Lemma LiftRcR Γ Γ' Γ'' τ (r : Ren Γ' Γ'') (r' : Ren Γ Γ') :
-  RTmL (τ := τ) (RcR r r') = RcR (RTmL r) (RTmL r').
+Lemma RcR_idRen_right {Γ Γ'} (σ : Ren Γ Γ') :
+  RcR σ idRen = σ.
 Proof.
-  extensionality τ'.
-  extensionality v.
-  now dependent elimination v.
+  induction σ; simp RcR; simpl; simp RcR; auto;
+  now rewrite IHσ.
 Qed.
 
-Corollary tlRen_skip1 Γ Γ' τ (f : Ren (τ :: Γ') Γ) :
-  tlRen f = RcR f skip1.
-Proof. reflexivity. Qed.
+Lemma RcR_assoc {Γ Γ' Γ'' Γ'''}
+      (σ : Ren Γ'' Γ''') (δ : Ren Γ' Γ'') (ν : Ren Γ Γ') :
+  RcR (RcR σ δ) ν = RcR σ (RcR δ ν).
+Proof.
+  generalize dependent Γ'''.
+  generalize dependent Γ''.
+  induction ν; simp RcR; simpl; intros; auto.
+  - simp RcR.
+    now rewrite IHν.
+  - dependent elimination δ; simp RcR; simpl.
+    + now rewrite IHν.
+    + dependent elimination σ; simp RcR; simpl;
+      now rewrite IHν.
+Qed.
 
-Corollary RcR_idRen_left Γ Γ' (f : Ren Γ' Γ) :
-  RcR idRen f = f.
-Proof. reflexivity. Qed.
+Equations RenVar {τ Γ Γ'} (r : Ren Γ Γ') (v : Var Γ' τ) : Var Γ τ :=
+  RenVar NoRen    v      := v;
+  RenVar (Drop σ) v      := SV (RenVar σ v);
+  RenVar (Keep σ) ZV     := ZV;
+  RenVar (Keep σ) (SV v) := SV (RenVar σ v).
 
-Corollary RcR_idRen_right Γ Γ' (f : Ren Γ' Γ) :
-  RcR f idRen = f.
-Proof. reflexivity. Qed.
+Lemma RenVar_idRen {τ Γ} (v : Var Γ τ) :
+  RenVar idRen v = v.
+Proof.
+  induction v; simpl; simp RenVar; intros; auto.
+  now rewrite IHv.
+Qed.
 
-Corollary RcR_assoc Γ Γ' Γ'' Γ'''
-          (f : Ren Γ' Γ) (g : Ren Γ'' Γ') (h : Ren Γ''' Γ'') :
-  RcR f (RcR g h) = RcR (RcR f g) h.
-Proof. reflexivity. Qed.
+Lemma RenVar_skip1 {τ τ' Γ} (v : Var Γ τ) :
+  RenVar (skip1 (τ:=τ')) v = SV v.
+Proof.
+  unfold skip1; simp RenVar.
+  now rewrite RenVar_idRen.
+Qed.
 
-Fixpoint RTmExp {Γ Γ' τ} (r : Ren Γ Γ') (e : Exp Γ τ) : Exp Γ' τ :=
+Lemma RenVar_RcR {τ Γ Γ' Γ''} (σ : Ren Γ' Γ'') (δ : Ren Γ Γ') (v : Var Γ'' τ) :
+  RenVar (RcR σ δ) v = RenVar δ (RenVar σ v).
+Proof.
+  generalize dependent Γ''.
+  induction δ; simpl; simp RcR; intros; auto.
+  - simp RenVar.
+    now rewrite <- IHδ.
+  - dependent elimination σ; simpl; simp RcR; simp RenVar.
+    + now rewrite IHδ.
+    + dependent elimination v; simp RenVar; auto.
+      now rewrite IHδ.
+Qed.
+
+Lemma Keep_RcR Γ Γ' Γ'' τ (r : Ren Γ' Γ'') (r' : Ren Γ Γ') :
+  Keep (τ := τ) (RcR r r') = RcR (Keep r) (Keep r').
+Proof.
+  generalize dependent Γ''.
+  now induction r'.
+Qed.
+
+Fixpoint RenExp {Γ Γ' τ} (r : Ren Γ Γ') (e : Exp Γ' τ) : Exp Γ τ :=
   match e with
   | Constant lit  => Constant lit
   | EUnit         => EUnit
   | ETrue         => ETrue
   | EFalse        => EFalse
-  | If b t e      => If (RTmExp r b) (RTmExp r t) (RTmExp r e)
-  | Pair x y      => Pair (RTmExp r x) (RTmExp r y)
-  | Fst p         => Fst (RTmExp r p)
-  | Snd p         => Snd (RTmExp r p)
-  | Seq exp1 exp2 => Seq (RTmExp r exp1) (RTmExp r exp2)
-  | Let x body    => Let (RTmExp r x) (RTmExp (RTmL r) body)
+  | If b t e      => If (RenExp r b) (RenExp r t) (RenExp r e)
+  | Pair x y      => Pair (RenExp r x) (RenExp r y)
+  | Fst p         => Fst (RenExp r p)
+  | Snd p         => Snd (RenExp r p)
+  | Seq exp1 exp2 => Seq (RenExp r exp1) (RenExp r exp2)
+  | Let x body    => Let (RenExp r x) (RenExp (Keep r) body)
 
-  | VAR v         => VAR (r _ v)
-  | APP e1 e2     => APP (RTmExp r e1) (RTmExp r e2)
-  | LAM e         => LAM (RTmExp (RTmL r) e)
+  | VAR v         => VAR (RenVar r v)
+  | APP e1 e2     => APP (RenExp r e1) (RenExp r e2)
+  | LAM e         => LAM (RenExp (Keep r) e)
   end.
 
-Lemma RTmExp_preserves_size {Γ Γ' τ} (r : Ren Γ Γ') (e : Exp Γ τ) :
-  Exp_size (RTmExp r e) = Exp_size e.
+Lemma RenExp_preserves_size {Γ Γ' τ} (r : Ren Γ Γ') (e : Exp Γ' τ) :
+  Exp_size (RenExp r e) = Exp_size e.
 Proof.
   generalize dependent r.
-  generalize dependent Γ'.
-  now induction e; simpl; intros; auto.
+  generalize dependent Γ.
+  now induction e; simpl; simp RcR; simpl; intros; auto.
 Qed.
 
-Definition wk {Γ τ τ'} : Exp Γ τ → Exp (τ' :: Γ) τ := RTmExp (λ _, SV).
-
-Lemma ActionRcR {Γ Γ' Γ''} (r : Ren Γ' Γ'') (r' : Ren Γ Γ') `(e : Exp Γ τ) :
-  RTmExp (RcR r r') e = RTmExp r (RTmExp r' e).
+Lemma RenExp_idRen {τ Γ} (e : Exp Γ τ) :
+  RenExp idRen e = e.
 Proof.
-  generalize dependent r'.
-  generalize dependent r.
-  generalize dependent Γ''.
+  induction e; simpl; simp RenVar; simpl; intros; auto;
+  rewrite ?IHe, ?IHe1, ?IHe2, ?IHe3; auto.
+  - now rewrite Keep_idRen, IHe2.
+  - now rewrite RenVar_idRen.
+  - now rewrite Keep_idRen, IHe.
+Qed.
+
+Lemma RenExp_RcR {τ Γ Γ' Γ''} (σ : Ren Γ' Γ'') (δ : Ren Γ Γ') (e : Exp Γ'' τ) :
+  RenExp (RcR σ δ) e = RenExp δ (RenExp σ e).
+Proof.
   generalize dependent Γ'.
+  generalize dependent Γ.
   induction e; simpl; intros; auto;
   rewrite ?IHe, ?IHe1, ?IHe2, ?IHe3; auto.
-  - rewrite LiftRcR.
-    now rewrite IHe2.
-  - rewrite LiftRcR.
-    now rewrite IHe.
+  - now rewrite <- IHe2; simp RcR.
+  - now rewrite RenVar_RcR.
+  - now rewrite <- IHe; simp RcR.
 Qed.
+
+Definition wk {Γ τ τ'} : Exp Γ τ → Exp (τ' :: Γ) τ := RenExp skip1.
 
 Definition identity Γ τ : Exp Γ (τ ⟶ τ) := LAM (VAR ZV).
 
-(** Now that we have renaming, we can define composition. *)
+(** Now that we have weakening, we can define composition. *)
 
-Definition compose {Γ τ τ' τ''}
+Definition composition {Γ τ τ' τ''}
            (f : Exp Γ (τ' ⟶ τ''))
            (g : Exp Γ (τ ⟶ τ')) : Exp Γ (τ ⟶ τ'') :=
   LAM (APP (wk f) (APP (wk g) (VAR ZV))).
